Examples.lean
@@ -1,3 +1,4 @@
 import Examples.Pow.Correct
 import Examples.Truth.Correct
 import Examples.Caller.Correct
+import Examples.ERC20.Correct
